squashme

TabularTypeInterpreter/Interpreter/Elaboration.lean
@@ -1,4 +1,5 @@
 import Lott.Data.Option
+import TabularTypeInterpreter.Data.List
 import TabularTypeInterpreter.Interpreter.«λπι»
 import TabularTypeInterpreter.Interpreter.Basic
 
@@ -27,7 +28,7 @@ def subst (τ τ' : Monotype) (i : TId) : Monotype := match τ with
   | uvar x => uvar x
   | lam i' κ τ'' => lam i' κ <| if i == i' then τ'' else subst τ'' τ' i
   | app ϕ τ'' => app (subst ϕ τ' i) (subst τ'' τ' i)
-  | arr τ₀ τ₁ => app (subst τ₀ τ' i) (subst τ₁ τ' i)
+  | arr τ₀ τ₁ => arr (subst τ₀ τ' i) (subst τ₁ τ' i)
   | label s => label s
   | floor ξ => floor <| subst ξ τ' i
   | comm u => comm u
@@ -54,12 +55,13 @@ decreasing_by
     · assumption
   )
 
+@[simp]
 def solve (τ τ' : Monotype) (x : UId) : Monotype := match τ with
   | var i => var i
   | uvar x' => if x == x' then τ' else uvar x'
   | lam i κ τ'' => lam i κ <| solve τ'' τ' x
   | app ϕ τ'' => app (solve ϕ τ' x) (solve τ'' τ' x)
-  | arr τ₀ τ₁ => app (solve τ₀ τ' x) (solve τ₁ τ' x)
+  | arr τ₀ τ₁ => arr (solve τ₀ τ' x) (solve τ₁ τ' x)
   | label s => label s
   | floor ξ => floor <| solve ξ τ' x
   | comm u => comm u
@@ -86,9 +88,32 @@ decreasing_by
     · assumption
   )
 
+theorem solve_subst_distrib
+  : solve (subst τ τ' i) τ'' x = subst (solve τ τ'' x) (solve τ' τ'' x) i := by
+  sorry
+
 def multiSubst (τ : Monotype) : List (Monotype × TId) → Monotype
 | [] => τ
-| (τ', i) :: iτ's => τ.subst τ' i |>.multiSubst iτ's
+| (τ', i) :: τ'is => τ.subst τ' i |>.multiSubst τ'is
+
+theorem multiSubst_append
+  : multiSubst (multiSubst τ τ'is) τ''is = multiSubst τ (τ'is ++ τ''is) := by
+  cases τ'is with
+  | nil => rw [multiSubst, List.nil_append]
+  | cons => rw [multiSubst, List.cons_append, multiSubst, multiSubst_append]
+
+theorem solve_multiSubst_distrib : solve (multiSubst τ τis) τ' x =
+    multiSubst (solve τ τ' x) (τis.map fun (τ, i) => (solve τ τ' x, i)) := by
+  rcases τis.cases_snoc with rfl | ⟨_, _, rfl⟩
+  · rw [multiSubst, List.map_nil, multiSubst]
+  · rw [← multiSubst_append, List.map_append, List.map_singleton, ← multiSubst_append, multiSubst,
+        multiSubst, solve_subst_distrib, solve_multiSubst_distrib, multiSubst, multiSubst]
+termination_by sizeOf τis
+decreasing_by
+  rename τis = _ => eq
+  subst eq
+  apply List.sizeOf_lt_sizeOf_append_right
+  simp_arith
 
 inductive CommutativityPartialOrdering : Monotype → Monotype → Prop where
   | refl : CommutativityPartialOrdering μ μ
@@ -108,7 +133,7 @@ instance : Decidable (CommutativityPartialOrdering μ₀ μ₁) :=
     | comm => nomatch hcomm
 
 theorem CommutativityPartialOrdering.solve
-  : CommutativityPartialOrdering μ₀ μ₁ → CommutativityPartialOrdering (μ₀.solve x τ) (μ₁.solve x τ)
+  : CommutativityPartialOrdering μ₀ μ₁ → CommutativityPartialOrdering (μ₀.solve τ x) (μ₁.solve τ x)
   | .refl => .refl
   | .non => by
     rw [Monotype.solve]
@@ -160,7 +185,7 @@ def sumElab : RowEquivalence ρ₀ μ ρ₁ → ElabM «λπι».Term
       let i ← freshId
       return .lam i <| .sumIntro (ξτs₁.findIdx (·.fst == ξ₀)) <| .var i
 
-def solve : RowEquivalence ρ₀ μ ρ₁ → RowEquivalence (ρ₀.solve x τ) (μ.solve x τ) (ρ₁.solve x τ)
+def solve : RowEquivalence ρ₀ μ ρ₁ → RowEquivalence (ρ₀.solve τ x) (μ.solve τ x) (ρ₁.solve τ x)
   | .refl => .refl
   | .trans re₀₁ re₁₂ => re₀₁.solve.trans re₁₂.solve
   | .comm perm => by
@@ -170,20 +195,20 @@ def solve : RowEquivalence ρ₀ μ ρ₁ → RowEquivalence (ρ₀.solve x τ) 
     rw [Monotype.solve, Monotype.solve, List.mapMem_eq_map, Monotype.solve, List.mapMem_eq_map,
         Monotype.solve, List.map_map,
         List.map_eq_map_iff (f := _ ∘ _)
-          (g := (fun (ξ, τ') => (ξ, ((ϕ.solve x τ).app τ'))) ∘
-            (fun (ξ, τ') => (ξ.solve x τ, τ'.solve x τ))) (l := ξτs).mpr (by
+          (g := (fun (ξ, τ') => (ξ, ((ϕ.solve τ x).app τ'))) ∘
+            (fun (ξ, τ') => (ξ.solve τ x, τ'.solve τ x))) (l := ξτs).mpr (by
           intros
-          simp [Monotype.solve]
+          simp
         ), ← List.map_map]
     exact .liftL
   | .liftR (ϕ := ϕ) (ξτs := ξτs) => by
     rw [Monotype.solve, Monotype.solve, List.mapMem_eq_map, Monotype.solve, List.mapMem_eq_map,
         Monotype.solve, List.map_map,
         List.map_eq_map_iff (f := _ ∘ _)
-          (g := (fun (ξ, τ') => (ξ, ((ϕ.solve x τ).app τ'))) ∘
-            (fun (ξ, τ') => (ξ.solve x τ, τ'.solve x τ))) (l := ξτs).mpr (by
+          (g := (fun (ξ, τ') => (ξ, ((ϕ.solve τ x).app τ'))) ∘
+            (fun (ξ, τ') => (ξ.solve τ x, τ'.solve τ x))) (l := ξτs).mpr (by
           intros
-          simp [Monotype.solve]
+          simp
         ), ← List.map_map]
     exact .liftR
 
@@ -267,22 +292,24 @@ def _root_.Nat.mapM [Monad m] : Nat → (Nat → m α) → m (List α)
 
 variable (TC)
 
-def ConstraintSolution.elab : ConstraintSolution τ → ElabM «λπι».Term
+namespace ConstraintSolution
+
+def «elab» : ConstraintSolution τ → ElabM «λπι».Term
   | «local» i => return .var i
-  | containTrans contain₀₁ce contain₁₂ce => do
-    let E ← contain₀₁ce.elab
-    let F ← contain₁₂ce.elab
+  | containTrans contain₀₁cs contain₁₂cs => do
+    let E ← contain₀₁cs.elab
+    let F ← contain₁₂cs.elab
     let i₀ ← freshId
     let i₁ ← freshId
     return .prodIntro [
       .lam i₀ <| (E.prodElim 0).app <| (F.prodElim 0).app <| .var i₀,
       .lam i₁ <| (F.prodElim 1).app <| (E.prodElim 1).app <| .var i₁,
     ]
-  | containConcat concat₂ce concat₅ce containₗce containᵣce => do
-    let E₂ ← concat₂ce.elab
-    let E₅ ← concat₅ce.elab
-    let Fₗ ← containₗce.elab
-    let Fᵣ ← containᵣce.elab
+  | containConcat concat₂cs concat₅cs containₗcs containᵣcs => do
+    let E₂ ← concat₂cs.elab
+    let E₅ ← concat₅cs.elab
+    let Fₗ ← containₗcs.elab
+    let Fᵣ ← containᵣcs.elab
     let i₀ ← freshId
     let i₁ ← freshId
     let i₂ ← freshId
@@ -327,10 +354,10 @@ def ConstraintSolution.elab : ConstraintSolution τ → ElabM «λπι».Term
         .lam i₅ <| .sumElim (.var i₅) [],
       ],
     ]
-  | concatAssocL concat₀₁ce concat₁₂ce concat₀₄ce => do
-    let E₀₁ ← concat₀₁ce.elab
-    let E₁₂ ← concat₁₂ce.elab
-    let E₀₄ ← concat₀₄ce.elab
+  | concatAssocL concat₀₁cs concat₁₂cs concat₀₄cs => do
+    let E₀₁ ← concat₀₁cs.elab
+    let E₁₂ ← concat₁₂cs.elab
+    let E₀₄ ← concat₀₄cs.elab
     let i₀ ← freshId
     let i₁ ← freshId
     let i₂ ← freshId
@@ -363,10 +390,10 @@ def ConstraintSolution.elab : ConstraintSolution τ → ElabM «λπι».Term
           ((E₁₂.prodElim 3).prodElim 1).app <| .var i₉,
       ],
     ]
-  | concatAssocR concat₀₁ce concat₁₂ce concat₃₂ce => do
-    let E₀₁ ← concat₀₁ce.elab
-    let E₁₂ ← concat₁₂ce.elab
-    let E₃₂ ← concat₃₂ce.elab
+  | concatAssocR concat₀₁cs concat₁₂cs concat₃₂cs => do
+    let E₀₁ ← concat₀₁cs.elab
+    let E₁₂ ← concat₁₂cs.elab
+    let E₃₂ ← concat₃₂cs.elab
     let i₀ ← freshId
     let i₁ ← freshId
     let i₂ ← freshId
@@ -404,8 +431,8 @@ def ConstraintSolution.elab : ConstraintSolution τ → ElabM «λπι».Term
           (E₃₂.prodElim 3).prodElim 1,
       ],
     ]
-  | concatSwap concatce => do
-    let E ← concatce.elab
+  | concatSwap concatcs => do
+    let E ← concatcs.elab
     let i₀ ← freshId
     let i₁ ← freshId
     let i₂ ← freshId
@@ -416,28 +443,28 @@ def ConstraintSolution.elab : ConstraintSolution τ → ElabM «λπι».Term
       E.prodElim 3,
       E.prodElim 2,
     ]
-  | concatContainL concatce => return .prodElim 2 <| ← concatce.elab
-  | concatContainR concatce => return .prodElim 3 <| ← concatce.elab
-  | containDecay containce _ => containce.elab
-  | concatDecay concatce _ => concatce.elab
-  | liftContain containce => containce.elab
-  | liftConcat concatce => concatce.elab
-  | tcInst { prereqs, mids, memberElab, superclassElab, .. } τ's ψsce => do
-    let Fs ← prereqs.mapMemM fun _ mem => ψsce _ mem |>.elab
+  | concatContainL concatcs => return .prodElim 2 <| ← concatcs.elab
+  | concatContainR concatcs => return .prodElim 3 <| ← concatcs.elab
+  | containDecay containcs _ => containcs.elab
+  | concatDecay concatcs _ => concatcs.elab
+  | liftContain containcs => containcs.elab
+  | liftConcat concatcs => concatcs.elab
+  | tcInst { prereqs, mids, memberElab, superclassElab, .. } τ's ψscs => do
+    let Fs ← prereqs.mapMemM fun _ mem => ψscs _ mem |>.elab
     return .prodIntro <| (memberElab.multiSubst (Fs.zip (mids.map (fun | { val } => { val })))) ::
       superclassElab.map fun Eₛ => Eₛ.multiSubst <| Fs.zip <| mids.map fun | { val } => { val }
-  | tcSuper tcτce n => return .prodElim n.succ <| ← tcτce.elab
+  | tcSuper tcτcs n => return .prodElim n.succ <| ← tcτcs.elab
   | allEmpty => return .unit
-  | allSingletonIntro ϕτce => return .prodIntro [← ϕτce.elab]
-  | allSingletonElim allce => return .prodElim 0 <| ← allce.elab
-  | allContain containce allce => do
-    let F ← containce.elab
-    let E ← allce.elab
+  | allSingletonIntro ϕτcs => return .prodIntro [← ϕτcs.elab]
+  | allSingletonElim allcs => return .prodElim 0 <| ← allcs.elab
+  | allContain containcs allcs => do
+    let F ← containcs.elab
+    let E ← allcs.elab
     return F.prodElim 0 |>.app E
-  | allConcat concatce all₀ce all₁ce => do
-    let F ← concatce.elab
-    let E₀ ← all₀ce.elab
-    let E₁ ← all₁ce.elab
+  | allConcat concatcs all₀cs all₁cs => do
+    let F ← concatcs.elab
+    let E₀ ← all₀cs.elab
+    let E₁ ← all₁cs.elab
     return F.prodElim 0 |>.app E₀ |>.app E₁
   | ind (ξτs := ξτs) => do
     let i₀ ← freshId
@@ -449,8 +476,8 @@ def ConstraintSolution.elab : ConstraintSolution τ → ElabM «λπι».Term
   | splitEmpty => concatConcrete 0 0
   | splitSingletonMatch => concatConcrete 1 0
   | splitSingletonRest => concatConcrete 0 1
-  | splitPiecewise _ _ _ _ _ concatce => concatce.elab
-  | splitConcat splitce => splitce.elab
+  | splitPiecewise _ _ _ _ _ concatcs => concatcs.elab
+  | splitConcat splitcs => splitcs.elab
 where
   concatConcrete (m n : Nat) : ElabM «λπι».Term := do
     let i₀ ← freshId
@@ -486,6 +513,156 @@ where
       ],
     ]
 
+def solve (cs : ConstraintSolution ψ) : ConstraintSolution (ψ.solve τ x) := by
+  cases cs with
+  | «local» i => exact .local i
+  | containTrans contain₀₁cs contain₁₂cs =>
+    replace contain₀₁cs := contain₀₁cs.solve (τ := τ) (x := x)
+    replace contain₁₂cs := contain₁₂cs.solve (τ := τ) (x := x)
+    rw [Monotype.solve] at contain₀₁cs contain₁₂cs ⊢
+    exact containTrans contain₀₁cs contain₁₂cs
+  | containConcat concat₂cs concat₅cs containₗcs containᵣcs =>
+    replace concat₂cs := concat₂cs.solve (τ := τ) (x := x)
+    replace concat₅cs := concat₅cs.solve (τ := τ) (x := x)
+    replace containₗcs := containₗcs.solve (τ := τ) (x := x)
+    replace containᵣcs := containᵣcs.solve (τ := τ) (x := x)
+    rw [Monotype.solve] at concat₂cs concat₅cs
+    rw [Monotype.solve] at containₗcs containᵣcs ⊢
+    exact containConcat concat₂cs concat₅cs containₗcs containᵣcs
+  | concatConcrete =>
+    simp
+    exact concatConcrete
+  | concatEmptyL =>
+    simp
+    exact concatEmptyL
+  | concatEmptyR =>
+    simp
+    exact concatEmptyR
+  | concatAssocL concat₀₁cs concat₁₂cs concat₀₄cs =>
+    replace concat₀₁cs := concat₀₁cs.solve (τ := τ) (x := x)
+    replace concat₁₂cs := concat₁₂cs.solve (τ := τ) (x := x)
+    replace concat₀₄cs := concat₀₄cs.solve (τ := τ) (x := x)
+    rw [Monotype.solve] at concat₀₁cs concat₁₂cs concat₀₄cs ⊢
+    exact concatAssocL concat₀₁cs concat₁₂cs concat₀₄cs
+  | concatAssocR concat₀₁cs concat₁₂cs concat₃₂cs =>
+    replace concat₀₁cs := concat₀₁cs.solve (τ := τ) (x := x)
+    replace concat₁₂cs := concat₁₂cs.solve (τ := τ) (x := x)
+    replace concat₃₂cs := concat₃₂cs.solve (τ := τ) (x := x)
+    rw [Monotype.solve] at concat₀₁cs concat₁₂cs concat₃₂cs ⊢
+    exact concatAssocR concat₀₁cs concat₁₂cs concat₃₂cs
+  | concatSwap concatcs =>
+    replace concatcs := concatcs.solve (τ := τ) (x := x)
+    simp at concatcs ⊢
+    exact concatSwap concatcs
+  | concatContainL concatcs =>
+    replace concatcs := concatcs.solve (τ := τ) (x := x)
+    simp at concatcs ⊢
+    exact concatContainL concatcs
+  | concatContainR concatcs =>
+    replace concatcs := concatcs.solve (τ := τ) (x := x)
+    simp at concatcs ⊢
+    exact concatContainR concatcs
+  | containDecay containcs po =>
+    replace containcs := containcs.solve (τ := τ) (x := x)
+    replace po := po.solve (τ := τ) (x := x)
+    simp at containcs po ⊢
+    exact containDecay containcs po
+  | concatDecay concatcs po =>
+    replace concatcs := concatcs.solve (τ := τ) (x := x)
+    replace po := po.solve (τ := τ) (x := x)
+    simp at concatcs po ⊢
+    exact concatDecay concatcs po
+  | liftContain containcs =>
+    replace containcs := containcs.solve (τ := τ) (x := x)
+    simp at containcs ⊢
+    exact liftContain containcs
+  | liftConcat concatcs =>
+    replace concatcs := concatcs.solve (τ := τ) (x := x)
+    simp at concatcs ⊢
+    exact liftConcat concatcs
+  | tcInst inst τ's ψscs =>
+    -- tids : List TId
+    -- prereqs : List Monotype
+    -- mids : List MId
+    -- name : String
+    -- target : Monotype
+    -- memberElab : «λπι».Term
+    -- superclassElab : List «λπι».Term
+    let { tids, prereqs, mids, name, target, memberElab, superclassElab } := inst
+    simp [Monotype.solve_multiSubst_distrib]
+    rw [List.zip_eq_zipWith, List.map_zipWith,
+        ← List.zipWith_map_left (f := fun τ' => Monotype.solve τ' τ x)]
+    apply tcInst {
+      prereqs := prereqs.map (·.solve τ x)
+      mids
+      target := _
+      memberElab
+      superclassElab
+      ..
+    } _
+    intro ψ mem
+    -- simp at mem
+    -- rcases List.mem_map.mp mem with ⟨_, mem', rfl⟩
+    let f := ψscs ψ sorry |>.solve (τ := τ) (x := x)
+    rw [solve_multiSubst_distrib] at f
+    simp at f ⊢
+    rw [List.zip_eq_zipWith, List.map_zipWith,
+        ← List.zipWith_map_left (f := fun τ' => Monotype.solve τ' τ x), ← List.zip_eq_zipWith] at f
+    sorry
+  | tcSuper tcτcs n =>
+    replace tcτcs := tcτcs.solve (τ := τ) (x := x)
+    rw [Monotype.solve, Monotype.solve] at tcτcs ⊢
+    exact tcSuper tcτcs n
+  | allEmpty =>
+    simp
+    exact allEmpty
+  | allSingletonIntro ϕτcs =>
+    replace ϕτcs := ϕτcs.solve (τ := τ) (x := x)
+    simp at ϕτcs ⊢
+    exact allSingletonIntro ϕτcs
+  | allSingletonElim allcs =>
+    replace allcs := allcs.solve (τ := τ) (x := x)
+    simp at allcs ⊢
+    exact allSingletonElim allcs
+  | allContain containcs allcs =>
+    replace containcs := containcs.solve (τ := τ) (x := x)
+    replace allcs := allcs.solve (τ := τ) (x := x)
+    simp at containcs allcs ⊢
+    exact allContain containcs allcs
+  | allConcat concatcs all₀cs all₁cs =>
+    replace concatcs := concatcs.solve (τ := τ) (x := x)
+    replace all₀cs := all₀cs.solve (τ := τ) (x := x)
+    replace all₁cs := all₁cs.solve (τ := τ) (x := x)
+    simp at concatcs all₀cs all₁cs ⊢
+    exact allConcat concatcs all₀cs all₁cs
+  | ind =>
+    rw [Monotype.solve]
+    exact ind
+  | splitEmpty =>
+    simp
+    exact splitEmpty
+  | splitSingletonMatch =>
+    simp
+    exact splitSingletonMatch
+  | splitSingletonRest =>
+    simp
+    exact splitSingletonRest
+  | splitPiecewise split₂cs split₅cs concat₆cs concat₇cs concat₈cs concatcs =>
+    replace split₂cs := split₂cs.solve (τ := τ) (x := x)
+    replace split₅cs := split₅cs.solve (τ := τ) (x := x)
+    replace concat₆cs := concat₆cs.solve (τ := τ) (x := x)
+    replace concat₇cs := concat₇cs.solve (τ := τ) (x := x)
+    replace concat₈cs := concat₈cs.solve (τ := τ) (x := x)
+    replace concatcs := concatcs.solve (τ := τ) (x := x)
+    simp at split₂cs split₅cs concat₆cs concat₇cs concat₈cs concatcs ⊢
+    exact splitPiecewise split₂cs split₅cs concat₆cs concat₇cs concat₈cs concatcs
+  | splitConcat concatcs =>
+    replace concatcs := concatcs.solve (τ := τ) (x := x)
+    simp at concatcs ⊢
+    exact splitConcat concatcs
+
+end ConstraintSolution
+
 end Monotype
 
 open Monotype
@@ -496,6 +673,7 @@ def subst (γ : QualifiedType) (τ : Monotype) (i : TId) : QualifiedType := matc
   | .mono τ' => τ'.subst τ i
   | .qual ψ γ' => subst γ' τ i |>.qual <| ψ.subst τ i
 
+@[simp]
 def solve (γ : QualifiedType) (τ : Monotype) (x : UId) : QualifiedType := match γ with
   | .mono τ' => τ'.solve τ x
   | .qual ψ γ' => solve γ' τ x |>.qual <| ψ.solve τ x
@@ -511,6 +689,7 @@ def subst (σ : TypeScheme) (τ : Monotype) (i : TId) : TypeScheme := match σ w
   | .quant i' κ σ' =>
     .quant i' κ <| if i == i' then σ' else subst σ' τ i
 
+@[simp]
 def solve (σ : TypeScheme) (τ : Monotype) (x : UId) : TypeScheme := match σ with
   | .qual γ => γ.solve τ x
   | .quant i κ σ' => .quant i κ <| solve σ' τ x
@@ -544,7 +723,9 @@ inductive Subtyping : TypeScheme → TypeScheme → Type where
   | list {τ₀ τ₁ : Monotype} : Subtyping τ₀ τ₁ →
     Subtyping (list.app τ₀) (list.app τ₁)
 
-def Subtyping.elab : Subtyping σ₀ σ₁ → ElabM «λπι».Term
+namespace Subtyping
+
+def «elab» : Subtyping σ₀ σ₁ → ElabM «λπι».Term
   | refl | decay _ => return .id
   | trans σ₀₁'st σ₁'₂st => do
     let i ← freshId
@@ -610,6 +791,35 @@ where
         .lam i'' <| (← ρ₁₃re.sumElab).app <| .app (.var i) <| (← ρ₀₂re.symm.sumElab).app <| .var i''
       ]
 
+def solve : Subtyping σ₀ σ₁ → Subtyping (σ₀.solve τ x) (σ₁.solve τ x)
+  | refl => refl
+  | trans σ₀₁'st σ₁'₂st => trans σ₀₁'st.solve σ₁'₂st.solve
+  | arr st st' => by
+    replace st := st.solve (τ := τ) (x := x)
+    replace st' := st'.solve (τ := τ) (x := x)
+    simp at st st' ⊢
+    exact arr st st'
+  | qual st st' => by
+    replace st := st.solve (τ := τ) (x := x)
+    replace st' := st'.solve (τ := τ) (x := x)
+    simp at st st' ⊢
+    exact qual st st'
+  | schemeL st' => sorry
+  | schemeR st' => sorry
+  | prodOrSum τ₀₁sst (Ξ := Ξ) (τ₀s := τ₀s) (τ₁s := τ₁s) => sorry
+  | prodOrSumRow ρ₀₁re (Ξ := Ξ) => sorry
+  | decay _ => sorry
+  | never => by
+    simp
+    exact never
+  | contain ρ₀₂re ρ₁₃re => sorry
+  | concat ρ₀₃re ρ₁₄re ρ₂₅re => sorry
+  | all ρ₀₁re => sorry
+  | split concatst => sorry
+  | list τ₀₁st => sorry
+
+end Subtyping
+
 end TypeScheme
 
 open TypeScheme
@@ -619,6 +829,36 @@ def «λπι».Op.result : «λπι».Op → Monotype
   | .eq | .lt | .le | .gt | .ge => .bool
 
 namespace Term
+
+@[simp]
+def solve (M : Term) (τ : Monotype) (x : UId) : Term := match M with
+  | var i => var i
+  | member s => member s
+  | lam i M' => lam i <| solve M' τ x
+  | app M' N => app (solve M' τ x) (solve N τ x)
+  | «let» i σ? M' N => «let» i (σ?.map (·.solve τ x)) (solve M' τ x) (solve N τ x)
+  | annot M' σ => annot (solve M' τ x) (σ.solve τ x)
+  | label s => label s
+  | prod M'Ns => prod <| M'Ns.mapMem fun (M', N) _ => (solve M' τ x, solve N τ x)
+  | sum M' N => sum (solve M' τ x) (solve N τ x)
+  | unlabel M' N => unlabel (solve M' τ x) (solve N τ x)
+  | prj M' => prj <| solve M' τ x
+  | concat M' N => concat (solve M' τ x) (solve N τ x)
+  | inj M' => inj <| solve M' τ x
+  | elim M' N => elim (solve M' τ x) (solve N τ x)
+  | ind ϕ ρ l t rn ri rp M' N =>
+    ind (ϕ.solve τ x) (ρ.solve τ x) l t rn ri rp (solve M' τ x) (solve N τ x)
+  | splitₚ ϕ M' => splitₚ (ϕ.solve τ x) (solve M' τ x)
+  | splitₛ ϕ M' N => splitₛ (ϕ.solve τ x) (solve M' τ x) (solve N τ x)
+  | nil => nil
+  | cons M' N => cons (solve M' τ x) (solve N τ x)
+  | fold i iₐ => fold i iₐ
+  | int i => int i
+  | op o M' N => op o (solve M' τ x) (solve N τ x)
+  | range => range
+  | str s => str s
+  | throw => throw
+  | «def» s => «def» s
 
 -- Existence of this Typing term doesn't actually prove the Term has this type; this is only used to
 -- guide elaboration, so it is up to the function producing this to ensure it is constructed
@@ -682,7 +922,9 @@ inductive Typing : Term → TypeScheme → Type where
 instance [Inhabited α] : Inhabited (Thunk α) where
   default := .mk fun _ => default
 
-def Typing.elab : Typing M σ → ReaderT (HashMap String «λπι».Term) ElabM «λπι».Term
+namespace Typing
+
+def «elab» : Typing M σ → ReaderT (HashMap String «λπι».Term) ElabM «λπι».Term
   | var (n := n) => return .var n
   | lam (i := i) M'ty => M'ty.elab <&> .lam i
   | app M'ty Nty => return (← M'ty.elab).app <| ← Nty.elab
@@ -726,6 +968,24 @@ def Typing.elab : Typing M σ → ReaderT (HashMap String «λπι».Term) ElabM
   | str (s := s) => return .str s
   | throw => return .throw
   | «def» (s := s) => return (← read)[s]!
+
+def solve (ty : Typing M σ) : Typing (M.solve τ x) (σ.solve τ x) := by
+  cases ty
+  · case var =>
+    simp
+    exact var
+  · case lam M'ty =>
+    replace M'ty := M'ty.solve (τ := τ) (x := x)
+    simp at M'ty ⊢
+    exact lam M'ty
+  · case app M'ty Nty =>
+    replace M'ty := M'ty.solve (τ := τ) (x := x)
+    replace Nty := Nty.solve (τ := τ) (x := x)
+    simp at M'ty Nty ⊢
+    exact app M'ty Nty
+  all_goals sorry
+
+end Typing
 
 end Term
 
